src/common/Coquplib.v
@@ -47,6 +47,7 @@ Ltac clear_obvious :=
   repeat match goal with
          | [ H : ex _ |- _ ] => invert H
          | [ H : ?C _ = ?C _ |- _ ] => invert H
+         | [ H : _ /\ _ |- _ ] => invert H
          end.
 
 Ltac simplify := simpl in *; clear_obvious; simpl in *; try discriminate.
@@ -79,6 +80,12 @@ Definition bind {A B : Type} (f : option A) (g : A -> option B) : option B :=
   match f with
   | Some a => g a
   | _ => None
+  end.
+
+Definition join {A : Type} (a : option (option A)) : option A :=
+  match a with
+  | None => None
+  | Some a' => a'
   end.
 
 Module Notation.
